src/PlutusIR/Semantics/Static/Typing_sound_complete.v
@@ -4,25 +4,6 @@ Import ListNotations.
 Require Import Coq.Bool.Bool.
 Require Import Coq.Strings.String.
 
-Inductive odd : nat -> Prop := oddS : forall n:nat, even n -> odd (S n)
-with even : nat -> Prop :=
-  | evenO : even 0
-  | evenS : forall n:nat, odd n -> even (S n).
-
-Scheme odd_even := Minimality for odd Sort Prop
-with even_odd := Minimality for even Sort Prop.
-
-Lemma even_plus_two : forall n, even n -> even (S (S n)).
-  intros.
-  induction even_odd with (P := odd) (P0 := (even)) (n := n) in H; intuition.
-  - apply evenS. apply oddS. apply evenO.
-  - apply evenS. apply oddS. assumption.
-  - apply oddS. assumption.
-  - apply evenO.
-  - apply evenS. assumption.
-Qed.
-
-
 From PlutusCert Require Import 
     Normalisation.Normalisation 
     Strong_normalisation
@@ -32,7 +13,8 @@ From PlutusCert Require Import
     Util.List
     Static.Util
     Equality
-    Kinding.Checker.
+    Kinding.Checker
+    Util.
 
 
 (** Typing of terms *)
@@ -108,10 +90,14 @@ Inductive has_type : list (string * kind) -> list (string * ty) -> term -> ty ->
       Δ' ,, Γ' |-+ t : Tn ->
       Δ |-* Tn : Kind_Base ->
       Δ ,, Γ |-+ (Let NonRec bs t) : Tn
-  | T_LetRec : forall Δ Γ b bs t, (* temp letrec definition for testing completeness*)
-      Δ ,, Γ |-ok_b b -> (* this is more like nonrec now that we do not update Δ and Γ*)
-      Δ ,, Γ |-+ (Let Rec (b :: bs) t) : Ty_Int
-
+  | T_LetRec : forall Δ Γ bs t Tn Δ' Γ' bsGn,
+      Δ' = flatten (map binds_Delta bs) ++ Δ ->
+      map_normalise (flatten (map binds_Gamma bs)) bsGn ->
+      Γ' = bsGn ++ Γ->
+      Δ' ,, Γ' |-oks_r bs ->
+      Δ' ,, Γ' |-+ t : Tn ->
+      Δ |-* Tn : Kind_Base ->
+      Δ ,, Γ |-+ (Let Rec bs t) : Tn
 (* Constructors are well-formed if their result type equals the fully applied
  * datatype (the last index), and all parameter types are well-kinded
 *)
@@ -158,12 +144,48 @@ with binding_well_formed : list (string * kind) -> list (string * ty) -> binding
   and "Δ ',,' Γ '|-oks_r' bs" := (bindings_well_formed_rec Δ Γ bs)
   and "Δ ',,' Γ '|-ok_b' b" := (binding_well_formed Δ Γ b).
 
+Scheme has_type_mut_ind := Induction for has_type Sort Prop
+with bs_wf_mut_ind := Induction for bindings_well_formed_rec Sort Prop
+with bs_wf_nonrec_mut_ind := Induction for bindings_well_formed_nonrec Sort Prop
+with b_wf_mut_ind := Induction for binding_well_formed Sort Prop.
 
-Fixpoint allb (bs : list bool) : bool :=
+Fixpoint allbmap {A : Type} (f : A -> bool) (bs : list A) : bool :=
     match bs with
     | [] => true
-    | b::bs => andb b (allb bs)
+    | b::bs => andb (f b) (allbmap f bs)
     end.
+
+Lemma allb_element_true : forall A f bs b, In b bs -> @allbmap A f bs = true -> f b = true.
+Proof.
+  intros.
+  induction bs.
+  - inversion H.
+  - simpl in H0.
+    destruct H.
+    + subst.
+      simpl in H0.
+      apply andb_true_iff in H0.
+      destruct H0.
+      assumption.
+    + apply andb_true_iff in H0.
+      destruct H0.
+      apply IHbs; auto.
+Qed.
+
+Lemma allbmap_each : forall A f bs, (forall b, In b bs -> f b = true) -> @allbmap A f bs = true.
+Proof.
+  intros.
+  induction bs.
+  - simpl. reflexivity.
+  - simpl.
+    apply andb_true_iff.
+    split.
+    + apply H. left. reflexivity.
+    + apply IHbs.
+      intros.
+      apply H.
+      right. assumption.
+Qed.
 
 Definition is_KindBase (k : option kind) : bool :=
   match k with 
@@ -174,17 +196,19 @@ Definition is_KindBase (k : option kind) : bool :=
 Definition constructor_well_formed_check (Δ : list (binderTyname * kind)) (v : vdecl) (Tr : ty ) : bool :=
   match v with
   | VarDecl x T => let (targs, tr') := splitTy T in
-          Ty_eqb Tr tr' && allb (map (fun U => is_KindBase (kind_check Δ U)) targs)
+          Ty_eqb Tr tr' && allbmap (fun U => is_KindBase (kind_check Δ U)) targs
   end.
 
 
-(* Idea Jacco: pass the recursively called type_check function as an argument even though it is not defined yet *)
+(* Idea Jacco: pass the recursively called type_check function as an argument even though it is not defined yet 
+Make another version that already has type_check as argument after type_check is defined.
+*)
 Definition binding_well_formed_check 
   (type_check' : ((list (binderTyname * kind)) -> (list (binderName * ty)) -> term -> option ty)) 
   (Δ : list (binderTyname * kind)) (Γ : list (binderName * ty)) binding : bool :=
     match binding with
     | (TypeBind (TyVarDecl X K) T) => match kind_check Δ T with
-                                      | Some K => true (* is this K the same as in the pattern match to the left? it should be*)
+                                      | Some K' => Kind_eqb K K' (* is this K the same as in the pattern match to the left? it should be*)
                                       | _ => false
                                       end
     | (TermBind s (VarDecl x T) t) => match kind_check Δ T with
@@ -200,7 +224,7 @@ Definition binding_well_formed_check
                                       end
     | (DatatypeBind (Datatype X YKs matchFunc cs)) => 
       let Δ' := rev (map fromDecl YKs) ++ Δ in
-      allb (map (fun c => constructor_well_formed_check Δ' c (constrLastTyExpected (Datatype X YKs matchFunc cs))) cs)
+      allbmap (fun c => constructor_well_formed_check Δ' c (constrLastTyExpected (Datatype X YKs matchFunc cs))) cs
     end.
 
 (* first argument represents binding_well_formed with the type_check already passed in *)
@@ -216,7 +240,7 @@ Definition bindings_well_formed_nonrec_check :
               b_wf Δ Γ b && f ((binds_Delta b) ++ Δ) (bsGn ++ Γ) bs'
             | _ => false
             end
-      | [] => true
+      | _ => true
     end.
 
 Definition bindings_well_formed_rec_check : (binding -> bool) -> list binding -> bool :=
@@ -227,7 +251,7 @@ Definition bindings_well_formed_rec_check : (binding -> bool) -> list binding ->
       | _ => true
     end.
 
-Fixpoint type_check (Δ : list (binderTyname * kind)) (Γ : list (binderName * ty)) (term : term) : (option ty) :=
+Fixpoint type_check (Δ : list (binderTyname * kind)) (Γ : list (binderName * ty)) (term : term) {struct term} : (option ty) :=
     match term with
     | Var x => lookup x Γ >>= fun T => normaliser_Jacco T
     | LamAbs x T1 t => 
@@ -286,11 +310,11 @@ Fixpoint type_check (Δ : list (binderTyname * kind)) (Γ : list (binderName * t
         let T := lookupBuiltinTy f in
         normaliser_Jacco T >>= fun Tn =>
         Some Tn
-    | Error S' => Some Ty_Int (* arbitrary! this will be sound but not complete *)
-    | Let NonRec (b::bs) t =>
+    | Error S' => Some Ty_Int (* arbitrary! this will be sound but not complete (zie teams Jacco over preservation type errors (app case))*)
+    | Let NonRec bs t =>
         let Δ' := flatten (map binds_Delta bs) ++ Δ in
         map_normaliser (flatten (map binds_Gamma bs)) >>= fun bsgn =>
-        let Γ' := flatten (map binds_Gamma bs) ++ Γ in
+        let Γ' := bsgn ++ Γ in
         if (bindings_well_formed_nonrec_check (binding_well_formed_check type_check) Δ Γ bs) then 
           type_check Δ' Γ' t >>= fun T =>
             match kind_check Δ T with
@@ -298,7 +322,7 @@ Fixpoint type_check (Δ : list (binderTyname * kind)) (Γ : list (binderName * t
             | _ => None
             end
         else None
-    (* | Let Rec bs t => (* Final let rec version*)
+    | Let Rec bs t => (* Final let rec version*)
         let Δ' := flatten (map binds_Delta bs) ++ Δ in
         map_normaliser (flatten (map binds_Gamma bs)) >>= fun bsgn =>
         let Γ' := bsgn ++ Γ in
@@ -308,57 +332,336 @@ Fixpoint type_check (Δ : list (binderTyname * kind)) (Γ : list (binderName * t
               | Some Kind_Base => Some T
               | _ => None
                 end 
-          else None *)
-    | Let Rec (b::bs) t =>
-        if (binding_well_formed_check type_check Δ Γ b) then Some Ty_Int else None  (* Temporarily easier efinition with only one bind check. To see how completeness works*)
-         
-    | _ => None
+          else None
+    | _ => None (* TODO: Case and Constr?? *)
     end.
 
-Theorem type_checking_sound : forall Δ Γ t ty,
-  type_check Δ Γ t = Some ty -> (Δ ,, Γ |-+ t : ty).
-Proof with (try apply kind_checking_sound; try apply normaliser_Jacco_sound; auto).
+Section term_recursivity_rect.
+  Variable (P : term -> Type).
+  Variable (Q : binding -> Type).
+  Variable (R : list binding -> Type).
+  Variable (S : list binding -> Type).
+
+  Context
+    (* (H_Let     : forall rec bs t, ForallT Q bs -> P t -> P (Let rec bs t)) *)
+    (H_LetRec     : forall bs t, R bs -> P t -> P (Let Rec bs t))
+    (H_LetNonRec  : forall bs t, S bs -> P t -> P (Let NonRec bs t))
+    (H_Var     : forall s, P (Var s))
+    (H_TyAbs   : forall s (k : kind) (t : term), P t -> P (TyAbs s k t))
+    (H_LamAbs  : forall s t (t0 : term), P t0 -> P (LamAbs s t t0))
+    (H_Apply   : forall t : term, P t -> forall t0 : term, P t0 -> P (Apply t t0))
+    (H_Constant : forall (c : constant), P (Constant c))
+    (H_Builtin : forall d : DefaultFun, P (Builtin d))
+    (H_TyInst  : forall t : term, P t -> forall t0 : ty, P (TyInst t t0))
+    (H_Error   : forall t : ty, P (Error t))
+    (H_IWrap   : forall (t t0 : ty) (t1 : term), P t1 -> P (IWrap t t0 t1))
+    (H_Unwrap  : forall t : term, P t -> P (Unwrap t))
+    (H_Constr  : forall (i : nat) T (ts : list (term)), ForallT P ts -> P (Constr i T ts))
+    (H_Case   : forall T t, P t -> forall ts, ForallT P ts -> P (Case T t ts)).
+
+  Context
+    (H_TermBind    : forall s v t, P t -> Q (TermBind s v t))
+    (H_TypeBind    : forall v ty, Q (TypeBind v ty))
+    (H_DatatypeBind : forall dtd, Q (DatatypeBind dtd)).
+
+  Context
+    (H_cons        : forall b bs, Q b -> R bs -> R (b :: bs))
+    (H_nil         : R nil).
+
+  Context
+    (H_consS      : forall b bs, Q b -> S bs -> S (b :: bs))
+    (H_nilS       : S nil).
+
+  Definition bindings_rect'' (binding_rect'' : forall (b : binding), Q b) :=
+    fix bindings_rect'' bs :=
+    match bs return R bs with
+      | nil       => @H_nil
+      | cons b bs => @H_cons _ bs (binding_rect'' b) (bindings_rect'' bs)
+    end.
+
+  Definition bindings_nonrect'' (binding_rect'' : forall (b : binding), Q b) :=
+    fix bindings_nonrect'' bs :=
+    match bs return S bs with
+      | nil       => @H_nilS
+      | cons b bs => @H_consS _ bs (binding_rect'' b) (bindings_nonrect'' bs)
+    end.
+
+  Definition terms_rect'' (term_rect : forall (t : term), P t) :=
+    fix terms_rect' ts :=
+    match ts as p return ForallT P p with
+      | nil       => ForallT_nil
+      | cons t ts => ForallT_cons (term_rect t) (terms_rect' ts)
+    end.
+
+  Fixpoint term_rect'' (t : term) : P t :=
+    match t with
+      | Let Rec bs t    => @H_LetRec bs t (bindings_rect'' binding_rect'' bs) (term_rect'' t)
+      | Let NonRec bs t => @H_LetNonRec bs t (bindings_nonrect'' binding_rect'' bs) (term_rect'' t)
+      | Var n           => @H_Var n
+      | TyAbs n k t     => @H_TyAbs n k t (term_rect'' t)
+      | LamAbs n ty t   => @H_LamAbs n ty t (term_rect'' t)
+      | Apply s t       => @H_Apply s (term_rect'' s) t (term_rect'' t)
+      | TyInst t ty     => @H_TyInst t (term_rect'' t) ty
+      | IWrap ty1 ty2 t => @H_IWrap ty1 ty2 t (term_rect'' t)
+      | Unwrap t        => @H_Unwrap t (term_rect'' t)
+      | Error ty        => @H_Error ty
+      | Constant c      => @H_Constant c
+      | Builtin f       => @H_Builtin f
+      | Constr i T ts     => @H_Constr i T ts (terms_rect'' term_rect'' ts)
+      | Case T t ts      => @H_Case T t (term_rect'' t) ts (terms_rect'' term_rect'' ts)
+    end
+  with binding_rect'' (b : binding) : Q b :=
+    match b with
+      | TermBind s v t   => @H_TermBind s v t (term_rect'' t)
+      | TypeBind v ty    => @H_TypeBind v ty
+      | DatatypeBind dtd => @H_DatatypeBind dtd
+    end.
+End term_recursivity_rect.
+
+Lemma constructor_well_formed_sound : 
+  forall Δ c T, constructor_well_formed_check Δ c T = true -> Δ |-ok_c c : T.
+Proof. 
+intros.
+destruct c.
+inversion H.
+remember (splitTy t).
+destruct p as [targs tr'].
+apply andb_true_iff in H1.
+destruct H1.
+apply Ty_eqb_eq in H0.
+subst.
+eapply W_Con.
+- eauto.
+- simpl in H1.
   intros.
-  generalize dependent Γ.
-  generalize dependent Δ.
-  generalize dependent ty.
-  induction t;
-    intros ty Δ Γ Htc; 
-    inversion Htc as [Htc']; 
-    unfold bind in Htc'; 
-    repeat destruct_match; 
-    inversion Htc'; 
+  apply (allb_element_true ty _ _ _ H0) in H1.
+  unfold is_KindBase in H1.
+  repeat destruct_match.
+  subst.
+  now apply kind_checking_sound in Heqo.
+Qed.
+
+Lemma constructor_well_formed_complete : 
+  forall Δ c T, Δ |-ok_c c : T -> constructor_well_formed_check Δ c T = true.
+Proof.
+  intros.
+  destruct c.
+  inversion H.
+  subst.
+  simpl.
+  remember (splitTy t) as splitT.
+  destruct splitT as [targs' T'].
+  inversion H3.
+  subst.
+  apply andb_true_iff.
+  split.
+  - apply Ty_eqb_refl.
+  - apply allbmap_each.
+    intros.
+    unfold is_KindBase.
+    specialize (H5 b0 H0).
+    apply kind_checking_complete in H5.
+    rewrite H5.
+    reflexivity.
+Qed.
+
+Theorem type_checking_sound : 
+ forall Δ Γ t ty, type_check Δ Γ t = Some ty -> (Δ ,, Γ |-+ t : ty).
+Proof with (try apply kind_checking_sound; try apply normaliser_Jacco_sound; auto).
+  intros Δ Γ t ty.
+  revert Δ Γ ty.
+  eapply term_rect'' with 
+    (P := fun t => forall Δ Γ ty, type_check Δ Γ t = Some ty -> Δ,, Γ |-+ t : ty)
+    (Q := fun b => forall Δ Γ, binding_well_formed_check type_check Δ Γ b = true -> binding_well_formed Δ Γ b)
+    (R := fun bs => forall Δ Γ, bindings_well_formed_rec_check (binding_well_formed_check type_check Δ Γ) bs = true -> bindings_well_formed_rec Δ Γ bs)
+    (S := fun bs => forall Δ Γ, bindings_well_formed_nonrec_check (binding_well_formed_check type_check) Δ Γ bs = true -> bindings_well_formed_nonrec Δ Γ bs).
+    repeat destruct_match.
+  - (* Case: Let *)
+    intros ec bs t0.
+    intros P.
+    intros.
+      inversion H.
+      unfold bind in H1.
+      repeat destruct_match.
+      eapply T_LetRec.
+      * reflexivity.
+      * apply map_normaliser_sound. eauto.
+      * reflexivity.
+      * eapply t0; eauto.
+      * eapply P; eauto.
+        inversion H1.
+        subst.
+        auto.
+      * 
+        inversion H1.
+        subst.
+        apply kind_checking_sound in Heqo1.
+        assumption.
+  - (* Case Let NONRec*)
+    intros rec bs t0.
+    intros P.
+    intros.
+      inversion H.
+      unfold bind in H1.
+      repeat destruct_match.
+      eapply T_Let with (Δ' := flatten (map binds_Delta rec) ++ Δ).
+      * reflexivity.
+      * apply map_normaliser_sound. eauto.
+      * reflexivity.
+      * eapply t0; eauto. 
+      * apply P.
+        inversion H1.
+        subst.
+        auto.
+      * 
+        inversion H1.
+        subst.
+        apply kind_checking_sound in Heqo1.
+        assumption.
+  - intros. 
+    inversion H.
+    unfold bind in H1.
+    repeat destruct_match.
+    (* apply normaliser_Jacco_sound in H1. *)
+    eapply T_Var; eauto...
+  - intros. 
+    inversion H0.
+    unfold bind in H0.
+    repeat destruct_match.
+    inversion H2.
     subst.
-  - (* Let, later *) admit.
-  - (* Let later *) admit.
-  - apply T_Var with (T := t)...
-  - apply T_TyAbs...
-  - apply T_LamAbs...
-  - eapply T_Apply.
-    + eapply IHt1; eauto.
-    + eapply IHt2; eauto.
+    eapply T_TyAbs...
+  - intros.
+    inversion H0.
+    unfold bind in H2.
+    repeat destruct_match.
+    inversion H2.
+    subst.
+    apply T_LamAbs...
+  - intros.
+    inversion H1.
+    unfold bind in H3.
+    repeat destruct_match.
+    inversion H3.
+    subst.
+    eapply T_Apply.
+    + eapply H; eauto.
+    + eapply H0; eauto.
       apply Ty_eqb_eq in Heqb.
       now subst.
-  - apply T_Constant.
-  - apply normaliser_Jacco_sound in Heqo.
+  - intros.
+    inversion H.
+    unfold bind in H1.
+    repeat destruct_match.
+    inversion H1; subst.
+    apply T_Constant.
+  - intros.
+    inversion H.
+    unfold bind in H1.
+    repeat destruct_match.
+    inversion H1; subst.
+    apply normaliser_Jacco_sound in Heqo.
     now apply T_Builtin with (T := lookupBuiltinTy d).
-  - apply Kind_eqb_eq in Heqb0.
+  - intros. inversion H0. unfold bind in H2. repeat destruct_match.
+    inversion H2. subst.
+    apply Kind_eqb_eq in Heqb0.
     subst.
-    apply T_TyInst with (X := b) (K2 := k0) (T1n := t2) (T2n := t3)...
-  - apply T_Error with (T := Ty_Int).
+    apply T_TyInst with (X := b) (K2 := k0) (T1n := t3) (T2n := t4)...
+  - intros.
+    inversion H. subst.
+    apply T_Error with (T := Ty_Int).
     + apply K_Builtin.
       apply K_DefaultUniInteger.
     + apply N_TyBuiltin.
-  - apply Ty_eqb_eq in Heqb0.
+  - intros.
+    inversion H0.
+    unfold bind in H2.
+    repeat destruct_match.
+    inversion H2.
+    subst.
+    apply Ty_eqb_eq in Heqb0.
     rewrite andb_true_iff in Heqb.
     destruct Heqb as [Heqb1 Heqb2].
     apply Kind_eqb_eq in Heqb1.
     apply Kind_eqb_eq in Heqb2.
-    inversion Htc'.
     subst.
-    apply T_IWrap with (K := k1_5) (T0n := t5)...
-  - apply T_Unwrap with (Fn := t1_1) (Tn := t1_2) (K := k)...
-Admitted.
+    apply T_IWrap with (K := k1_5) (T0n := t6)...
+  - intros.
+    inversion H0.
+    unfold bind in H2.
+    repeat destruct_match.
+    inversion H2. subst.
+    apply T_Unwrap with (Fn := t2_1) (Tn := t2_2) (K := k)...
+  - intros.
+    inversion H.
+  - intros.
+    inversion H0.
+  - intros.
+    inversion H0.
+    repeat destruct_match.
+    subst.
+    apply W_Term with (Tn := t3).
+    + apply kind_checking_sound in Heqo.
+      assumption.
+    + now apply normaliser_Jacco_sound in Heqo1.
+    + apply Ty_eqb_eq in H2.
+      subst.
+      eapply H; eauto.
+  - intros.
+    inversion H.
+    repeat destruct_match.
+    apply W_Type.
+    apply kind_checking_sound in Heqo.
+    apply Kind_eqb_eq in H1.
+    subst.
+    assumption.
+  - intros.
+    inversion H.
+    repeat destruct_match.
+    subst.
+    eapply W_Data.
+    * reflexivity.
+    * intros.
+      unfold constrLastTyExpected.
+      assert (constructor_well_formed_check (rev (map fromDecl l) ++ Δ) c (Ty_Apps (Ty_Var (getTyname t0)) (map (Ty_Var ∘ getTyname) l)) = true).
+      { eapply (allb_element_true) in H1.
+        - exact H1.
+        - assumption.
+       }
+      now apply constructor_well_formed_sound.
+  - intros.
+    apply W_ConsB_Rec.
+    + apply H.
+      inversion H1.
+      apply andb_true_iff in H3.
+      destruct H3.
+      rewrite H2.
+      rewrite H3.
+      auto.
+    + eapply H0.
+      inversion H1.
+      apply andb_true_iff in H3.
+      destruct H3.
+      rewrite H2.
+      rewrite H3.
+      auto.
+  - intros.
+    apply W_NilB_Rec.
+  - intros.
+    inversion H1.
+    destruct_match.
+    apply andb_true_iff in H3.
+    destruct H3.
+    eapply W_ConsB_NonRec.
+    + apply H.
+      assumption.
+    + apply map_normaliser_sound in Heqo.
+      eauto.
+    + apply H0.
+      assumption.
+  - intros.
+    apply W_NilB_NonRec.
+Qed.
 
 (* Hmmm, why does this rewrite?? This helper lemma is of course temporary TODO *)
 Lemma test (T2n T1n : ty) Δ Γ t x :
@@ -388,41 +691,84 @@ Theorem type_checking_complete : forall Δ Γ t ty,
     (Δ ,, Γ |-+ t : ty) -> type_check Δ Γ t = Some ty.
 Proof.
   intros.
-  induction b_wf__typing__rec in H.
-  induction H; simpl; auto.
-  - rewrite H.
-    now apply normaliser_Jacco_complete. 
-  - apply normaliser_Jacco_complete in H0; rewrite H0; simpl.
-    apply kind_checking_complete in H; rewrite H.
+  apply has_type_mut_ind with         
+        (P := fun Δ Γ t T _ => type_check Δ Γ t = Some T)
+        (P0 := fun Δ Γ l _ => bindings_well_formed_rec_check (binding_well_formed_check type_check Δ Γ) l = true) 
+        (P1 := fun Δ Γ l _ => bindings_well_formed_nonrec_check (binding_well_formed_check type_check) Δ Γ l = true )
+        (P2 := fun Δ Γ b _ => binding_well_formed_check type_check Δ Γ b = true) 
+        ; simpl; auto; intros.
+  - (*Case T_Var *)
+    rewrite e. simpl. 
+    now apply normaliser_Jacco_complete.
+  - (* Case: T_LamAbs *)
+     apply normaliser_Jacco_complete in n; rewrite n; simpl.
+    apply kind_checking_complete in h; rewrite h.
     (* rewrite IHhas_type. Why does this not work?? *)
     now apply test.
-  - rewrite IHhas_type1.
-    rewrite IHhas_type2.
+  - (* Case: T_Apply *)
+    rewrite H0.
+    rewrite H1.
     now rewrite -> Ty_eqb_refl.
-  - (* easy with a lemma like test *)
-    now apply oof2.        
-  - rewrite IHhas_type.
-    apply kind_checking_complete in H0; rewrite H0.
+  - (* Case: T_TyAbs *) 
+    now apply oof2.   
+  - (* Case: T_Inst *)
+    rewrite H0.
+    apply kind_checking_complete in h0; rewrite h0.
     rewrite -> Kind_eqb_refl.
-    apply normaliser_Jacco_complete in H1; rewrite H1; simpl.
-    now apply normaliser_Jacco_complete in H2; rewrite H2; simpl.
-  - apply kind_checking_complete in H; rewrite H.
-    apply kind_checking_complete in H1; rewrite H1.
-    rewrite IHhas_type.
+    apply normaliser_Jacco_complete in n; rewrite n; simpl.
+    now apply normaliser_Jacco_complete in n0; rewrite n0; simpl.
+  - (* Case T_IWrap *)
+    apply kind_checking_complete in h; rewrite h.
+    apply kind_checking_complete in h0; rewrite h0.
+    rewrite H0.
     rewrite Kind_eqb_refl; simpl.
-    apply normaliser_Jacco_complete in H0; rewrite H0; simpl.
-    apply normaliser_Jacco_complete in H2; rewrite H2; simpl.
-    apply normaliser_Jacco_complete in H3; rewrite H3; simpl.
+    apply normaliser_Jacco_complete in n; rewrite n; simpl.
+    apply normaliser_Jacco_complete in n0; rewrite n0; simpl.
+    apply normaliser_Jacco_complete in n1; rewrite n1; simpl.
     now rewrite Ty_eqb_refl.
-  - rewrite IHhas_type.
-    apply kind_checking_complete in H0; rewrite H0.
-    now apply normaliser_Jacco_complete in H1; rewrite H1; simpl.
-  - subst.
-    now apply normaliser_Jacco_complete in H0; rewrite H0; simpl.
-  - (* error case, not complete by implementation *) admit.
-  - (* let case: later *) admit.
-  - (* we dont have the necessary induction hypothesis, we need mutual recursive proof on binding_well_formed_check ? *)
-
+  - (* Case: T_Unwrap*)
+    rewrite H0.
+    apply kind_checking_complete in h0; rewrite h0.
+    now apply normaliser_Jacco_complete in n; rewrite n; simpl.
+  - (* Case: T_Builtin*)
+    subst.
+    now apply normaliser_Jacco_complete in n; rewrite n; simpl.
+  - (* Case: T_Error *)
+    admit. (* TODO: Not complete in current implementation*)
+  - (* Case: T_Let *)
+  (* Cas Let NonRec    (* apply map_normaliser_complete in m. *)
+    (* In the goal we need things about subterms of bs. That is probably fine here, but I'm not sure why and probably in soundness this will then go wrong?*)
+    admit. *)
+    apply map_normaliser_complete in m; rewrite m; simpl.
+    rewrite H0.
+    subst.
+    rewrite H1; simpl.
+    apply kind_checking_complete in h0; rewrite h0.
+    reflexivity.
+  - (* Case: T_LetRec *)
+    intros. simpl. subst.
+    apply map_normaliser_complete in m; rewrite m; simpl.
+    rewrite H0.
+    rewrite H1.
+    simpl.
+    apply kind_checking_complete in h0; rewrite h0. auto.
+  - (* Case: ? *)
+    intros. simpl. rewrite H0. auto.
+  - (* Case: ? *)
+    apply map_normaliser_complete in m; rewrite m.
+    intuition.
+  - intros. simpl. rewrite H0.
+    apply normaliser_Jacco_complete in n; rewrite n.
+    rewrite Ty_eqb_refl.
+    apply kind_checking_complete in h; rewrite h.
+    auto.
+  - intros. simpl. apply kind_checking_complete in h; rewrite h. auto. apply Kind_eqb_eq. reflexivity.
+  - intros. simpl. apply allbmap_each with (bs := cs).
+    intros.
+    specialize (c b H0).
+    apply constructor_well_formed_complete in c.
+    subst.
+    assumption.
 Admitted.
     
 
